1) phisubst_inv.v was proved. This proof is highly similar to id_rhs_val.v, at least 70% of which are exactly the same. The different proofs are at Lemmas wf_defs_updateAddAL and wf_defs_br_aux. In the two lemmas, most of the cases are also the same. We should generalize the proofs into subst_inv.v.
2) The similarity of proofs that can be generalized.
  a) Proofs based on SSA-property:
     Vellvm/opsem_wf.v Vellvm/opsem_dom.v Transforms/id_rhs_val.v 
     Transforms/alive_store.v Transforms/alive_alloca.v 
     Transforms/phisubst_inv.v

  b) Proofs based on liveness of memory locations.
     Transforms/alive_store.v Transforms/alive_alloca.v 

  c) Proofs about eliminating irrelevant memory contents
     Transforms/sas.v Transforms/dse.v Transforms/dae.v

  d) Proofs that based on the invariants proved by SSA-property (a)
     Transforms/promotable_props.v Trasforms/palloca_props.v
     which proved memory properties w.r.t SSA variables.

  e) Proofs that establish top-level coarse simulations from level-level 
     fine simulations.
     Transforms/???_top.v



git-svn-id: https://webdav.seas.upenn.edu/svn/sol/vol@3979 eef5ea85-cc2e-0410-bd84-0fae1f012da8

src3.0/Transforms/id_rhs_val.v
@@ -114,14 +114,6 @@ match v with
     end
 end.
 
-Definition substing_value (f:fdef) (v:value) : Prop :=
-match v with
-| value_const _ => True
-| value_id vid =>
-    In vid (getArgsIDsOfFdef f) \/
-    exists instr, lookupInsnViaIDFromFdef f vid = ret instr
-end.
-
 Definition substable_values TD gl (f:fdef) (v1 v2:value) : Prop :=
 substable_value f v1 /\ substing_value f v2 /\ valueDominates f v2 v1 /\
 match v1, v2 with
