src3.0/Transforms/phisubst_inv.v
@@ -1,30 +1,1020 @@
 Require Import vellvm.
+Require Import Maps.
+Require Import Lattice.
+Require Import opsem_props.
+Require Import trans_tactic.
 Require Import primitives.
 Require Import subst_inv.
 Require Import phielim_spec.
 
 Record PEInfo := mkPEInfo {
   PEI_f : fdef;
+  PEI_b : block;
   PEI_p : phinode;
   PEI_v : value;
-  PEI_lkup: lookupInsnViaIDFromFdef PEI_f (getPhiNodeID PEI_p) = 
-              Some (insn_phinode PEI_p);
+  PEI_in: phinodeInFdefBlockB PEI_p PEI_f PEI_b = true;
+  PEI_subst: substing_value PEI_f PEI_v;
   PEI_assign: assigned_phi PEI_v PEI_p
 }.
 
+Lemma PEInfo__domination: forall (pi:PEInfo) s m (HwfF: wf_fdef s m (PEI_f pi))
+  (Huniq: uniqFdef (PEI_f pi)),
+  valueDominates (PEI_f pi) (PEI_v pi) (value_id (getPhiNodeID (PEI_p pi))).
+Proof.
+  destruct pi.
+  simpl. intros.
+  destruct_phinodeInFdefBlockB_tac.
+  eapply assigned_phi__domination in PEI_assign0; eauto.
+Qed.
+
+Lemma PEInfo__lookupInsnViaIDFromFdef: forall (pi:PEInfo)
+  (Huniq: uniqFdef (PEI_f pi)),
+  lookupInsnViaIDFromFdef (PEI_f pi) (getPhiNodeID (PEI_p pi))
+    = Some (insn_phinode (PEI_p pi)).
+Proof.
+  destruct pi. simpl. intros.
+  destruct_phinodeInFdefBlockB_tac.
+  solve_lookupInsnViaIDFromFdef.
+Qed.
+
+Lemma PEInfo_p__isnt__cmd: forall (pi:PEInfo) (Huniq: uniqFdef (PEI_f pi))
+  l1 ps1 cs1 tmn1 c
+  (HBinF: blockInFdefB (block_intro l1 ps1 cs1 tmn1) (PEI_f pi) = true)
+  (Hin : In c cs1),
+  getCmdLoc c <> getPhiNodeID (PEI_p pi).
+Proof.
+  intros.
+  assert (Hlk:=Huniq).
+  apply PEInfo__lookupInsnViaIDFromFdef in Hlk.
+  eapply IngetCmdsIDs__lookupCmdViaIDFromFdef in HBinF; eauto.
+  intro EQ. rewrite EQ in *.
+  congruence.
+Qed.
+
+(* similar to id_rhs_val.v *)
+Lemma valueDominates_value_in_scope__value_in_scope__cmd: forall 
+  pi S M (c : cmd) (ids1 : list atom) (Huniq : uniqFdef (PEI_f pi))
+  (HwfF: wf_fdef S M (PEI_f pi)) 
+  (l1 : l) (ps1 : phinodes) (cs1 : cmds) (tmn1 : terminator)
+  (H : blockInFdefB (block_intro l1 ps1 cs1 tmn1) (PEI_f pi) = true)
+  (H0 : In c cs1)
+  (Hreach : isReachableFromEntry (PEI_f pi) (block_intro l1 ps1 cs1 tmn1))
+  (Hinscope : 
+    ret ids1 = inscope_of_cmd (PEI_f pi) (block_intro l1 ps1 cs1 tmn1) c)
+  ids2
+  (Heq : AtomSet.set_eq _ (getCmdLoc c::ids1) ids2)
+  (Hina : value_in_scope (value_id (getPhiNodeID (PEI_p pi))) ids2),
+  value_in_scope (PEI_v pi) ids2.
+Proof.
+Local Opaque inscope_of_cmd.
+  intros.
+  assert (Hdom:=HwfF). apply PEInfo__domination in Hdom; auto.
+  assert (Hval2:=PEI_subst pi).
+  destruct Heq as [Hinc1 Hinc2].
+  remember (PEI_v pi) as v2. 
+  destruct v2 as [vid2|]; auto.
+  apply Hinc1.
+  simpl. right.
+  assert (getCmdLoc c <> getPhiNodeID (PEI_p pi)) as Hneq.
+    eapply PEInfo_p__isnt__cmd; eauto.
+  assert (In (getPhiNodeID (PEI_p pi)) ids1) as Hinscope'.
+    apply Hinc2 in Hina. 
+    destruct_in Hina; try congruence.
+  assert (Hlkid:=Huniq). apply PEInfo__lookupInsnViaIDFromFdef in Hlkid.
+  assert (Hidreach:=Hinscope').
+  eapply inscope_of_cmd__id_in_reachable_block 
+    with (vid:=getPhiNodeID (PEI_p pi)) in Hidreach; eauto 1.
+  simpl.
+  apply Hdom in Hidreach; auto.
+  apply in_split in H0. destruct H0 as [cs3 [cs2 H0]]; subst.
+  destruct Hval2 as [Hval2 | [instr Hval2]].
+    eapply in_getArgsIDsOfFdef__inscope_of_cmd; eauto 1.
+    eapply idDominates_inscope_of_cmd__inscope_of_cmd; eauto 2.
+Transparent inscope_of_cmd.
+Qed.
+
+(* similar to id_rhs_val.v *)
+Lemma wf_defs_updateAddAL: forall (pi:PEInfo) td gl F' lc' c ids1 ids2 g0
+  s m (HwfF: wf_fdef s m F') (Huniq: uniqFdef F') l1 ps1 cs1 tmn1 
+  (H : blockInFdefB (block_intro l1 ps1 cs1 tmn1) F' = true)
+  (H0 : In c cs1) (Hreach: isReachableFromEntry F' (block_intro l1 ps1 cs1 tmn1))
+  (Hinscope: ret ids1 = inscope_of_cmd F' (block_intro l1 ps1 cs1 tmn1) c)
+  (Hinscope2' : wf_defs (value_id (getPhiNodeID (PEI_p pi))) (PEI_v pi) (PEI_f pi) 
+                  td gl F' lc' ids1)
+  (Hinscope2'' : OpsemPP.wf_defs td F' lc' ids1)
+  (Heq : AtomSet.set_eq _ (getCmdLoc c::ids1) ids2)
+  (Hsome: getCmdID c <> None),
+  wf_defs (value_id (getPhiNodeID (PEI_p pi))) (PEI_v pi) (PEI_f pi) 
+    td gl F' (updateAddAL _ lc' (getCmdLoc c) g0) ids2.
+Proof.
+Local Opaque inscope_of_cmd.
+  intros.
+  intros EQ gvsa gvsb Hina Hgeta Hgetb; subst.
+  assert (Hinb: value_in_scope (PEI_v pi) ids2).
+    eapply valueDominates_value_in_scope__value_in_scope__cmd; eauto.
+  destruct Heq as [Hinc1 Hinc2].
+  assert (Hdom:=HwfF). apply PEInfo__domination in Hdom; auto.
+  assert (getCmdLoc c <> getPhiNodeID (PEI_p pi)) as Hneq.
+    eapply PEInfo_p__isnt__cmd; eauto.
+  assert (In (getPhiNodeID (PEI_p pi)) ids1) as Hin.
+    apply Hinc2 in Hina. simpl in Hina.
+    destruct Hina; subst; try congruence; auto.
+  unfold wf_defs in Hinscope2'.
+  simpl in *.
+  remember (PEI_v pi) as v2.
+  destruct v2 as [vid2 | vc2]; simpl in *.
+    SCase "v2 = vid2".
+      rewrite <- lookupAL_updateAddAL_neq in Hgeta; auto.
+      destruct (vid2 == getCmdLoc c); subst.
+      SSSCase "vid2 == c".
+        (* vid1 in ids1 ==> vid1 >> c
+           vid2 == c ==> vid1 >> vid2. Cycle!! *)
+        elimtype False.
+        apply inscope_of_cmd__idDominates with 
+          (i0:=(getPhiNodeID (PEI_p pi))) in Hinscope; 
+          auto using in__cmdInBlockB.
+        assert (id_in_reachable_block (PEI_f pi) (getPhiNodeID (PEI_p pi))) 
+          as Hinv.
+          (* vid1 in scope, so it is reachable. *)
+          eapply OpsemPP.wf_defs_elim in Hinscope2''; eauto. tauto.
+        eapply idDominates_acyclic in Hinv; eauto.
+
+      SSSCase "vid2 <> c".
+        rewrite <- lookupAL_updateAddAL_neq in Hgetb; auto.
+
+    SCase "v2 = vc2".
+      rewrite <- lookupAL_updateAddAL_neq in Hgeta; auto.
+Transparent inscope_of_cmd.
+Qed.
+
+Ltac destruct_ctx_return :=
+match goal with
+| Hwfcfg : OpsemPP.wf_Config ?cfg,
+  Hwfpp : OpsemPP.wf_State ?cfg _,
+  HwfS1 : wf_State _ _ _ _ _ |- _ =>
+  destruct Hwfcfg as [_ [_ [HwfSystem HmInS]]];
+  destruct Hwfpp as 
+    [Hnempty [
+     [Hreach1 [HBinF1 [HFinPs1 [Hwflc1 [Hinscope1 [l1 [ps1 [cs1' Heq1]]]]]]]]
+     [
+      [
+        [Hreach2 [HBinF2 [HFinPs2 [Hwflc2 [Hinscope2 [l2 [ps2 [cs2' Heq2]]]]]]]]
+        [HwfECs HwfCall]
+      ]
+      HwfCall'
+     ]]
+    ]; subst;
+  fold (@OpsemPP.wf_ECStack DGVs) in HwfECs;
+  destruct HwfS1 as [Hinscope1' [Hinscope2' HwfECs']];
+  fold wf_ECStack in HwfECs';
+  unfold wf_ExecutionContext in Hinscope1', Hinscope2';
+  simpl in Hinscope1', Hinscope2'
+end.
+
+(* similar to id_rhs_val.v *)
+Lemma valueDominates_value_in_scope__value_in_scope__at_beginning: forall 
+  pi S M (ids1 : list atom) (Huniq : uniqFdef (PEI_f pi))
+  (HwfF: wf_fdef S M (PEI_f pi)) 
+  (l1 : l) (ps1 : phinodes) (cs1 : cmds) (tmn1 : terminator)
+  (H : blockInFdefB (block_intro l1 ps1 cs1 tmn1) (PEI_f pi) = true)
+  (Hreach : isReachableFromEntry (PEI_f pi) (block_intro l1 ps1 cs1 tmn1)) ids2
+  (contents' : ListSet.set atom)
+  (inbound' : incl contents' (bound_fdef (PEI_f pi)))
+  (Heqdefs' : {|
+             DomDS.L.bs_contents := contents';
+             DomDS.L.bs_bound := inbound' |} = (dom_analyze (PEI_f pi)) !! l1)
+  (Hinscope : (fold_left (inscope_of_block (PEI_f pi) l1) contents'
+    (ret (getPhiNodesIDs ps1 ++ getArgsIDsOfFdef (PEI_f pi))) = ret ids2))
+  (Hina : value_in_scope (value_id (getPhiNodeID (PEI_p pi))) ids2),
+  value_in_scope (PEI_v pi) ids2.
+Proof.
+  intros.
+  assert (Hdom:=HwfF). apply PEInfo__domination in Hdom; auto.
+  assert (Hval2:=PEI_subst pi).
+  remember (PEI_v pi) as v2. 
+  destruct v2 as [vid2|]; auto.
+  simpl in Hval2. 
+  assert (Hlkid:=Huniq). apply PEInfo__lookupInsnViaIDFromFdef in Hlkid.
+  assert (Hidreach:=Hreach). 
+  eapply inscope_of_blocks_with_init__id_in_reachable_block 
+    with (vid:=getPhiNodeID (PEI_p pi)) in Hidreach; eauto 1.
+    simpl.
+    apply Hdom in Hidreach; auto.
+    destruct Hval2 as [Hval2 | [instr Hval2]].
+      eapply in_getArgsIDsOfFdef__inscope_of_blocks_with_init; eauto.
+      intros x Hin. xsolve_in_list.
+
+      eapply idDominates_inscope_of_cmd_at_beginning__inscope_of_cmd_at_beginning;
+        eauto 2.
+
+    intros id0 Hin0. simpl.
+    destruct_in Hin0; xsolve_in_list.
+Qed.
+
+(* similar to id_rhs_val.v *)
+Lemma wf_defs_br_aux : forall pi TD gl S M lc l' ps' cs' lc' F tmn' l1 ps1 cs1 
+  tmn1 (HBinF: blockInFdefB (block_intro l1 ps1 cs1 tmn1) F = true)
+  (Hreach : isReachableFromEntry F (block_intro l1 ps1 cs1 tmn1))
+  (Hreach': isReachableFromEntry F (block_intro l' ps' cs' tmn'))
+  (Hlkup : Some (block_intro l' ps' cs' tmn') = lookupBlockViaLabelFromFdef F l')
+  (Hswitch : Opsem.switchToNewBasicBlock TD (block_intro l' ps' cs' tmn') 
+               (block_intro l1 ps1 cs1 tmn1) gl lc = ret lc')
+  (t : list atom)
+  (Hinscope': ret t = inscope_of_tmn F (block_intro l1 ps1 cs1 tmn1) tmn1)
+  (Hwfdfs : wf_defs (value_id (getPhiNodeID (PEI_p pi))) (PEI_v pi) (PEI_f pi) 
+             TD gl F lc t)
+  (Hwfdfs' : OpsemPP.wf_defs TD F lc t)
+  (ids0' : list atom)
+  (HwfF : wf_fdef S M F) (HuniqF: uniqFdef F)
+  (contents' : ListSet.set atom)
+  (inbound' : incl contents' (bound_fdef F))
+  (Heqdefs' : {|
+             DomDS.L.bs_contents := contents';
+             DomDS.L.bs_bound := inbound' |} = (dom_analyze F) !! l')
+  (Hinscope : (fold_left (inscope_of_block F l') contents'
+    (ret (getPhiNodesIDs ps' ++ getArgsIDsOfFdef F)) = ret ids0'))
+  (Hinc : incl (ListSet.set_diff eq_atom_dec ids0' (getPhiNodesIDs ps')) t),
+  wf_defs (value_id (getPhiNodeID (PEI_p pi))) (PEI_v pi) (PEI_f pi)  
+    TD gl F lc' ids0'.
+Proof.
+Local Opaque inscope_of_tmn.
+  intros. 
+  assert (HBinF':=Hlkup).
+  symmetry in HBinF'.
+  apply lookupBlockViaLabelFromFdef_inv in HBinF'; auto.
+  destruct HBinF' as [_ HBinF'].
+
+  intros EQ gvs1 gvs2 Hin1 Hget1 Hget2; subst.
+  assert (Hin2: value_in_scope (PEI_v pi) ids0').
+    eapply valueDominates_value_in_scope__value_in_scope__at_beginning 
+      in Hinscope; eauto 1.
+      solve_blockInFdefB.
+  assert (Hdom:=HwfF). apply PEInfo__domination in Hdom; auto.
+(* destruct Hvals as [Hval1 [Hval2 [Hdom _]]]. *)
+  unfold Opsem.switchToNewBasicBlock in Hswitch. simpl in Hswitch.
+  remember (Opsem.getIncomingValuesForBlockFromPHINodes TD ps' 
+              (block_intro l1 ps1 cs1 tmn1) gl lc) as R1.
+  destruct R1 as [rs|]; inv Hswitch.
+  simpl in *.
+  destruct (In_dec id_dec (getPhiNodeID (PEI_p pi)) (getPhiNodesIDs ps'))
+    as [Hpin1 | Hnotin1].
+  Case "p in ps".
+    assert (getPhiNodeID (PEI_p pi) `in` dom rs) as Hinrs.
+      eapply OpsemProps.getIncomingValuesForBlockFromPHINodes_spec6; eauto.
+    assert (match (PEI_v pi) with
+            | value_id vid0 => vid0 `notin` dom rs
+            | _ => True
+            end) as Hnotinrs.
+       destruct (PEI_v pi) as [vid0 | vc0]; auto.
+         eapply OpsemProps.getIncomingValuesForBlockFromPHINodes_spec8; eauto.
+         intro J.
+         eapply phinodes_from_the_same_block__dont__valueDominate in Hdom;
+           eauto 1.
+    apply OpsemProps.updateValuesForNewBlock_spec6 in Hget1; auto.
+    eapply OpsemProps.getIncomingValuesForBlockFromPHINodes_spec9' in HeqR1; 
+      eauto 1.
+    destruct HeqR1 as [t1 [vls1 [v [HinPs [Hnth Hget]]]]].
+    assert (insn_phi (getPhiNodeID (PEI_p pi)) t1 vls1 = PEI_p pi) as EQ.
+      assert (Hlkup':=HuniqF).
+      apply PEInfo__lookupInsnViaIDFromFdef in Hlkup'.
+      eapply IngetPhiNodesIDs__lookupPhinodeViaIDFromFdef' in HinPs; eauto 1.
+      simpl in *. uniq_result. auto.
+    assert (J:=PEI_assign pi).
+    rewrite <- EQ in J.
+    inv J.
+    assert (In (v, getBlockLabel (block_intro l1 ps1 cs1 tmn1)) vls1) as Hinlist.
+      apply getValueViaLabelFromValuels__InValueList; auto.
+    apply Hassign in Hinlist.
+    destruct Hinlist as [Hinlist | Hinlist]; subst.
+    SCase "reading PEI_p".
+      assert (In (getPhiNodeID (PEI_p pi)) t) as Hint.
+        assert (wf_phinode (PEI_f pi) (block_intro l' ps' cs' tmn')
+                 (insn_phi (getPhiNodeID (PEI_p pi)) t1 vls1)) as Hwfp.
+          eapply wf_fdef__wf_phinode; eauto.
+            solve_blockInFdefB.
+        eapply incoming_value__in_scope in Hinscope'; eauto 1.
+      assert (Opsem.getOperandValue TD (PEI_v pi) lc gl = ret gvs2) as Hget2'.
+        destruct (PEI_v pi) as [vid0 | vc0]; auto.
+          simpl in Hget2.
+          eapply OpsemProps.updateValuesForNewBlock_spec7 in Hget2; eauto.
+      eapply Hwfdfs in Hint; eauto.
+
+    SCase "reading PEI_v".
+      destruct (PEI_v pi) as [vid0 | vc0]; simpl in Hget2, Hget.
+        eapply OpsemProps.updateValuesForNewBlock_spec7 in Hget2; eauto.
+        congruence.
+
+        congruence.
+
+  Case "p notin ps".
+    assert (Hnotin1' := Hnotin1).
+    apply ListSet.set_diff_intro with (x:=ids0')(Aeq_dec:=eq_atom_dec)
+      in Hnotin1; auto.
+    apply Hinc in Hnotin1. assert (HeqR1':=HeqR1).
+    eapply OpsemProps.getIncomingValuesForBlockFromPHINodes_spec8 in HeqR1;
+      eauto.
+    eapply OpsemProps.updateValuesForNewBlock_spec7 in Hget1; eauto.
+
+    remember (PEI_v pi) as v2.
+    destruct v2 as [vid2 | vc2]; simpl in *; eauto.
+    SCase "v2 = vid2".
+      assert (~ In vid2 (getPhiNodesIDs ps')) as Hnotin2.
+        (* vid1 in ids0' /\ vid1 notin ps' /\ vid2 in ps' ==>  
+           v1d1 >> vid2 !! *)
+        intro Hin.
+        eapply inscope_of_cmd_at_beginning__idDominates__phinode
+          with (i0:=getPhiNodeID (PEI_p pi)) in Hinscope; eauto.
+        assert (id_in_reachable_block (PEI_f pi) (getPhiNodeID (PEI_p pi))) 
+          as Hinv.
+          (* vid1 in scope, so it is reachable. *)
+          eapply OpsemPP.wf_defs_elim in Hwfdfs'; eauto. tauto.
+        eapply idDominates_acyclic in Hinv; eauto. 
+
+      assert (Hnotin2' := Hnotin2).
+      apply ListSet.set_diff_intro with (x:=ids0')(Aeq_dec:=eq_atom_dec)
+        in Hnotin2; auto.
+      apply Hinc in Hnotin2. assert (HeqR1'':=HeqR1').
+      eapply OpsemProps.getIncomingValuesForBlockFromPHINodes_spec8 in HeqR1';
+        eauto.
+      eapply OpsemProps.updateValuesForNewBlock_spec7 in Hget2; eauto.
+Transparent inscope_of_tmn.
+Qed.
+
+(* similar to id_rhs_val.v *)
+Lemma inscope_of_tmn_br_aux : forall pi S M F l3 ps cs tmn ids0 l' ps' cs' tmn'
+  l0 lc lc' gl TD (Hreach : isReachableFromEntry F (block_intro l3 ps cs tmn))
+  (Hwfdfs': OpsemPP.wf_defs TD F lc ids0),
+wf_fdef S M F -> 
+uniqFdef F ->
+blockInFdefB (block_intro l3 ps cs tmn) F = true ->
+In l0 (successors_terminator tmn) ->
+Some ids0 = inscope_of_tmn F (block_intro l3 ps cs tmn) tmn ->
+Some (block_intro l' ps' cs' tmn') = lookupBlockViaLabelFromFdef F l0 ->
+Opsem.switchToNewBasicBlock TD (block_intro l' ps' cs' tmn')
+  (block_intro l3 ps cs tmn) gl lc = Some lc' ->
+wf_defs (value_id (getPhiNodeID (PEI_p pi))) (PEI_v pi) (PEI_f pi)  
+  TD gl F lc ids0 ->
+exists ids0',
+  match cs' with
+  | nil => Some ids0' = inscope_of_tmn F (block_intro l' ps' cs' tmn') tmn'
+  | c'::_ => Some ids0' = inscope_of_cmd F (block_intro l' ps' cs' tmn') c'
+  end /\
+  incl (ListSet.set_diff eq_atom_dec ids0' (getPhiNodesIDs ps')) ids0 /\
+  wf_defs (value_id (getPhiNodeID (PEI_p pi))) (PEI_v pi) (PEI_f pi)  
+    TD gl F lc' ids0'.
+Proof.
+  intros pi S M F l3 ps cs tmn ids0 l' ps' cs' tmn' l0 lc lc' gl TD Hreach Hwfdfs'
+    HwfF HuniqF HBinF Hsucc Hinscope Hlkup Hswitch Hwfdfs.
+  symmetry in Hlkup.
+  assert (J:=Hlkup).
+  apply lookupBlockViaLabelFromFdef_inv in J; auto.
+  destruct J as [Heq J]; subst.
+  assert (Hinscope':=Hinscope).
+  unfold inscope_of_tmn in Hinscope.
+  unfold inscope_of_tmn. unfold inscope_of_cmd, inscope_of_id.
+  destruct F as [fh bs].
+  remember (dom_analyze (fdef_intro fh bs)) as Doms.
+  remember (Doms !! l3)as defs3.
+  remember (Doms !! l')as defs'.
+  destruct defs3 as [contents3 inbound3].
+  destruct defs' as [contents' inbound'].
+
+  assert (incl contents' (l3::contents3)) as Hsub.
+    clear - HBinF Hsucc Heqdefs3 Heqdefs' HeqDoms HuniqF HwfF.
+    apply uniqF__uniqBlocks in HuniqF.
+    simpl in HuniqF.
+    eapply dom_successors; eauto.
+
+  assert (isReachableFromEntry (fdef_intro fh bs) (block_intro l' ps' nil tmn'))
+    as Hreach'.
+    eapply isReachableFromEntry_successors in Hlkup; eauto.
+
+  assert (J1:=inbound'). destruct fh as [f t i0 a v].
+  apply fold_left__bound_blocks with (init:=getPhiNodesIDs ps' ++
+    getArgsIDs a)(bs:=bs)(l0:=l') (fh:=fheader_intro f t i0 a v) in J1; auto.
+  destruct J1 as [r J1].
+  exists r. 
+
+  assert (incl (ListSet.set_diff eq_atom_dec r (getPhiNodesIDs ps')) ids0)
+    as Jinc.
+    clear - Hinscope J1 Hsub HBinF HuniqF.
+    eapply inscope_of_tmn__inscope_of_cmd_at_beginning in J1; eauto. 
+
+  destruct cs'.
+  Case "cs'=nil".
+    simpl.
+    split; auto.
+    split; auto.
+      subst. simpl in J1. simpl_env in J1.
+      eapply wf_defs_br_aux in Hswitch; eauto.
+  Case "cs'<>nil".
+    assert (~ In (getCmdLoc c) (getPhiNodesIDs ps')) as Hnotin.
+      apply uniqFdef__uniqBlockLocs in J; auto.
+      simpl in J. 
+      eapply NoDup_disjoint in J; simpl; eauto.
+    rewrite init_scope_spec1; auto.
+    unfold cmds_dominates_cmd. simpl.
+    destruct (eq_atom_dec (getCmdLoc c) (getCmdLoc c)) as [_ | n];
+      try solve [contradict n; auto].
+    split; auto.
+    split; auto.
+      subst. eapply wf_defs_br_aux in Hswitch; eauto.
+Qed.
+
+(* same to id_rhs_val.v *)
+Lemma inscope_of_tmn_br_uncond : forall pi S M F l3 ps cs ids0 l' ps' 
+  cs' tmn' l0 lc lc' bid TD gl
+  (Hwfdfs': OpsemPP.wf_defs TD F lc ids0),
+isReachableFromEntry F (block_intro l3 ps cs (insn_br_uncond bid l0)) ->
+wf_fdef S M F -> uniqFdef F ->
+blockInFdefB (block_intro l3 ps cs (insn_br_uncond bid l0)) F = true ->
+Some ids0 = inscope_of_tmn F (block_intro l3 ps cs (insn_br_uncond bid l0))
+  (insn_br_uncond bid l0) ->
+Some (block_intro l' ps' cs' tmn') = lookupBlockViaLabelFromFdef F l0 ->
+Opsem.switchToNewBasicBlock TD (block_intro l' ps' cs' tmn')
+  (block_intro l3 ps cs (insn_br_uncond bid l0)) gl lc = Some lc' ->
+wf_defs (value_id (getPhiNodeID (PEI_p pi))) (PEI_v pi) (PEI_f pi)  
+  TD gl F lc ids0 ->
+exists ids0',
+  match cs' with
+  | nil => Some ids0' = inscope_of_tmn F (block_intro l' ps' cs' tmn') tmn'
+  | c'::_ => Some ids0' = inscope_of_cmd F (block_intro l' ps' cs' tmn') c'
+  end /\
+  incl (ListSet.set_diff eq_atom_dec ids0' (getPhiNodesIDs ps')) ids0 /\
+  wf_defs (value_id (getPhiNodeID (PEI_p pi))) (PEI_v pi) (PEI_f pi) 
+    TD gl F lc' ids0'.
+Proof.
+  intros.
+  eapply inscope_of_tmn_br_aux; eauto.
+  simpl. auto.
+Qed.
+
+(* same to id_rhs_val.v *)
+Lemma inscope_of_tmn_br : forall pi S M F l0 ps cs bid l1 l2 ids0 l' 
+  ps' cs' tmn' Cond c lc lc' gl TD
+  (Hwfdfs': OpsemPP.wf_defs TD F lc ids0),
+isReachableFromEntry F (block_intro l0 ps cs (insn_br bid Cond l1 l2)) ->
+wf_fdef S M F -> uniqFdef F ->
+blockInFdefB (block_intro l0 ps cs (insn_br bid Cond l1 l2)) F = true ->
+Some ids0 = inscope_of_tmn F (block_intro l0 ps cs (insn_br bid Cond l1 l2))
+  (insn_br bid Cond l1 l2) ->
+Some (block_intro l' ps' cs' tmn') =
+       (if isGVZero TD c
+        then lookupBlockViaLabelFromFdef F l2
+        else lookupBlockViaLabelFromFdef F l1) ->
+Opsem.switchToNewBasicBlock TD (block_intro l' ps' cs' tmn')
+  (block_intro l0 ps cs (insn_br bid Cond l1 l2)) gl lc = Some lc' ->
+wf_defs (value_id (getPhiNodeID (PEI_p pi))) (PEI_v pi) (PEI_f pi) 
+  TD gl F lc ids0 ->
+exists ids0',
+  match cs' with
+  | nil => Some ids0' = inscope_of_tmn F (block_intro l' ps' cs' tmn') tmn'
+  | c'::_ => Some ids0' = inscope_of_cmd F (block_intro l' ps' cs' tmn') c'
+  end /\
+  incl (ListSet.set_diff eq_atom_dec ids0' (getPhiNodesIDs ps')) ids0 /\
+  wf_defs (value_id (getPhiNodeID (PEI_p pi))) (PEI_v pi) (PEI_f pi)
+    TD gl F lc' ids0'.
+Proof.
+  intros.
+  remember (isGVZero TD c) as R.
+  destruct R; eapply inscope_of_tmn_br_aux; eauto; simpl; auto.
+Qed.
+
+Ltac destruct_ctx_other :=
+match goal with
+| Hwfcfg : OpsemPP.wf_Config ?cfg,
+  Hwfpp : OpsemPP.wf_State ?cfg _,
+  HwfS1 : wf_State _ _ _ _ _ |- _ =>
+  destruct Hwfcfg as [_ [_ [HwfSystem HmInS]]];
+  destruct Hwfpp as 
+    [Hnempty [
+     [Hreach1 [HBinF1 [HFinPs1 [Hwflc1 [Hinscope1 [l1' [ps1' [cs1' Heq1]]]]]]]]
+     [HwfECs HwfCall]]
+    ]; subst;
+  fold (@OpsemPP.wf_ECStack DGVs) in HwfECs;
+  destruct HwfS1 as [Hinscope1' HwfECs'];
+  fold wf_ECStack in HwfECs';
+  unfold wf_ExecutionContext in Hinscope1';
+  simpl in Hinscope1'
+end.
+
+(* same to id_rhs_val.v *)
+Lemma preservation_cmd_updated_case : forall pi
+  (B : block)
+  lc gv3
+  (cs : list cmd)
+  (tmn : terminator)
+  id0 c0 los nts gl Mem0 Mem1 als EC fs Ps S
+  (Hid : Some id0 = getCmdID c0) Cfg St
+  (Hwfcfg : OpsemPP.wf_Config Cfg) (Hwfpp : OpsemPP.wf_State Cfg St)
+  (EQ1 : Cfg = {| OpsemAux.CurSystem := S;
+                  OpsemAux.CurTargetData := (los, nts);
+                  OpsemAux.CurProducts := Ps;
+                  OpsemAux.Globals := gl;
+                  OpsemAux.FunTable := fs |}) F0
+  (EQ2 : St = {| Opsem.ECS := {|
+                           Opsem.CurFunction := F0;
+                           Opsem.CurBB := B;
+                           Opsem.CurCmds := c0 :: cs;
+                           Opsem.Terminator := tmn;
+                           Opsem.Locals := lc;
+                           Opsem.Allocas := als |} :: EC;
+                 Opsem.Mem := Mem0 |})
+  (HwfS1 : wf_State (value_id (getPhiNodeID (PEI_p pi))) (PEI_v pi) 
+            (PEI_f pi) Cfg St) als',
+  wf_State (value_id (getPhiNodeID (PEI_p pi))) (PEI_v pi) (PEI_f pi) Cfg
+     {|
+     Opsem.ECS := {|
+            Opsem.CurFunction := F0;
+            Opsem.CurBB := B;
+            Opsem.CurCmds := cs;
+            Opsem.Terminator := tmn;
+            Opsem.Locals := updateAddAL _ lc id0 gv3;
+            Opsem.Allocas := als' |} :: EC;
+     Opsem.Mem := Mem1 |}.
+Proof.
+Local Opaque inscope_of_cmd inscope_of_tmn.
+  intros. subst.
+  destruct_ctx_other.
+  split; auto.
+    unfold wf_ExecutionContext. simpl.
+    remember (inscope_of_cmd F0 (block_intro l1' ps1' (cs1' ++ c0 :: cs) tmn) c0)
+      as R1.
+    assert (HeqR1':=HeqR1).
+    assert (uniqFdef F0) as HuniqF.
+      eapply wf_system__uniqFdef; eauto.
+    destruct R1; try solve [inversion Hinscope1].
+      assert (Hid':=Hid).
+      symmetry in Hid.
+      apply getCmdLoc_getCmdID in Hid.
+      subst.
+      assert (cmdInBlockB c0 (block_intro l1' ps1' (cs1' ++ c0 :: cs) tmn)
+               = true) as Hin.
+        simpl. apply In_InCmdsB. apply in_middle.
+      assert (NoDup (getBlockLocs (block_intro l1' ps1' (cs1' ++ c0 :: cs) tmn))) 
+        as Hnotin.
+        eapply wf_system__uniq_block with (f:=F0) in HwfSystem; eauto.
+      destruct cs; simpl_env in *.
+      Case "1.1.1".
+        apply inscope_of_cmd_tmn in HeqR1; auto.
+        destruct HeqR1 as [ids2 [J1 J2]].
+        rewrite <- J1.
+        assert (In c0 (cs1' ++ [c0])) as HinCs.
+          apply in_or_app. right. simpl. auto.
+        assert (Hwfc := HBinF1).
+        eapply wf_system__wf_cmd with (c:=c0) in Hwfc;
+          eauto.
+        rewrite <- Hid' in J2.
+        assert (HwfF:=HFinPs1). eapply wf_system__wf_fdef in HwfF; eauto.
+        eapply wf_defs_updateAddAL; try solve [eauto | congruence].
+
+      Case "1.1.2".
+        apply inscope_of_cmd_cmd in HeqR1; auto.
+        destruct HeqR1 as [ids2 [J1 J2]].
+        rewrite <- J1.
+        assert (In c0 (cs1' ++ [c0] ++ [c] ++ cs)) as HinCs.
+          apply in_or_app. right. simpl. auto.
+        assert (Hwfc := HBinF1).
+        eapply wf_system__wf_cmd with (c:=c0) in Hwfc;
+          eauto.
+        rewrite <- Hid' in J2.
+        assert (HwfF:=HFinPs1). eapply wf_system__wf_fdef in HwfF; eauto.
+        eapply wf_defs_updateAddAL; try solve [eauto | congruence].
+Transparent inscope_of_cmd inscope_of_tmn.
+Qed.
+
+(* same to id_rhs_val *)
+Lemma preservation_cmd_non_updated_case : forall pi
+  (S : system)
+  (los : layouts)
+  (nts : namedts)
+  (Ps : list product)
+  (B : block)
+  lc (gl : GVMap)
+  (fs : GVMap) EC
+  (cs : list cmd)
+  (tmn : terminator)
+  (Mem0 Mem1: mem)
+  (als : list mblock)
+  c0
+  (Hid : getCmdID c0 = None) Cfg St
+  (Hwfcfg : OpsemPP.wf_Config Cfg) (Hwfpp : OpsemPP.wf_State Cfg St)
+  (EQ1 : Cfg = {| OpsemAux.CurSystem := S;
+                  OpsemAux.CurTargetData := (los, nts);
+                  OpsemAux.CurProducts := Ps;
+                  OpsemAux.Globals := gl;
+                  OpsemAux.FunTable := fs |}) F0
+  (EQ2 : St = {| Opsem.ECS := {|
+                           Opsem.CurFunction := F0;
+                           Opsem.CurBB := B;
+                           Opsem.CurCmds := c0 :: cs;
+                           Opsem.Terminator := tmn;
+                           Opsem.Locals := lc;
+                           Opsem.Allocas := als |} :: EC;
+                 Opsem.Mem := Mem0 |})
+  (HwfS1 : wf_State (value_id (getPhiNodeID (PEI_p pi))) (PEI_v pi) 
+             (PEI_f pi) Cfg St),
+  wf_State (value_id (getPhiNodeID (PEI_p pi))) (PEI_v pi) (PEI_f pi) Cfg
+     {|
+     Opsem.ECS := {|
+            Opsem.CurFunction := F0;
+            Opsem.CurBB := B;
+            Opsem.CurCmds := cs;
+            Opsem.Terminator := tmn;
+            Opsem.Locals := lc;
+            Opsem.Allocas := als |} :: EC;
+     Opsem.Mem := Mem1 |}.
+Proof.
+Local Opaque inscope_of_cmd inscope_of_tmn.
+  intros. subst.
+  destruct_ctx_other.
+  split; auto.
+    remember (inscope_of_cmd F0 (block_intro l1' ps1' (cs1' ++ c0 :: cs) tmn) c0)
+      as R1.
+    destruct R1; try solve [inversion Hinscope1].
+    unfold wf_ExecutionContext. simpl.
+    assert (NoDup (getBlockLocs (block_intro l1' ps1' (cs1' ++ c0 :: cs) tmn))) 
+      as Hnotin.
+      eapply wf_system__uniq_block with (f:=F0) in HwfSystem; eauto.
+    destruct cs; simpl_env in *.
+    Case "1.1.1".
+        apply inscope_of_cmd_tmn in HeqR1; auto.
+        destruct HeqR1 as [ids2 [J1 J2]].
+        rewrite <- J1.
+        assert (In c0 (cs1' ++ [c0])) as HinCs.
+          apply in_or_app. right. simpl. auto.
+        assert (Hwfc := HBinF1).
+        eapply wf_system__wf_cmd with (c:=c0) in Hwfc;
+          eauto.
+        rewrite Hid in J2.
+        eapply wf_defs_eq; eauto.
+
+    Case "1.1.2".
+        apply inscope_of_cmd_cmd in HeqR1; auto.
+        destruct HeqR1 as [ids2 [J1 J2]].
+        rewrite <- J1.
+        assert (In c0 (cs1' ++ [c0] ++ [c] ++ cs)) as HinCs.
+          apply in_or_app. right. simpl. auto.
+        assert (Hwfc := HBinF1).
+        eapply wf_system__wf_cmd with (c:=c0) in Hwfc;
+          eauto.
+        rewrite Hid in J2.
+        eapply wf_defs_eq ; eauto.
+Transparent inscope_of_cmd inscope_of_tmn.
+Qed.
+
+Lemma PEInfo_p__isnt__arg: forall (pi:PEInfo) (Huniq: uniqFdef (PEI_f pi)),
+  ~ In (getPhiNodeID (PEI_p pi)) (getArgsIDsOfFdef (PEI_f pi)).
+Proof.
+  intros.
+  assert (Hlk:=Huniq).
+  apply PEInfo__lookupInsnViaIDFromFdef in Hlk.
+  solve_notin_getArgsIDs.
+Qed.
+
+(* similar to id_rhs_val *)
+Lemma preservation_dbCall_case : forall fid fa rt la va lb td lc gl
+  (Huniq: uniqFdef (fdef_intro (fheader_intro fa rt fid la va) lb)) pi,
+  wf_defs (value_id (getPhiNodeID (PEI_p pi))) (PEI_v pi) (PEI_f pi) td gl
+    (fdef_intro (fheader_intro fa rt fid la va) lb) lc (getArgsIDs la).
+Proof.
+  intros.
+  assert (incl nil (bound_blocks lb)) as J.
+    intros x J. inv J.
+  intros EQ gvs1 gvs2 Hin1 Hget1 Hget2; subst.
+  simpl in Hin1.
+  contradict Hin1.
+  rewrite <- EQ in Huniq.
+  apply PEInfo_p__isnt__arg in Huniq.
+  rewrite EQ in Huniq. auto.
+Qed.
+
+(* same to id_rhs_val *)
 Lemma preservation: forall (cfg1 : OpsemAux.Config)
   (S1 S1' : Opsem.State) (tr : trace) (pi: PEInfo)
   (Hcfg: OpsemPP.wf_Config cfg1) (Hpp: OpsemPP.wf_State cfg1 S1)
-  (Hop: Opsem.sInsn cfg1 S1 S1' tr)
-  (HwfS : subst_inv.wf_State (value_id (getPhiNodeID (PEI_p pi))) (PEI_v pi) 
+  (HsInsn: Opsem.sInsn cfg1 S1 S1' tr)
+  (HwfS1 : subst_inv.wf_State (value_id (getPhiNodeID (PEI_p pi))) (PEI_v pi) 
           (PEI_f pi) cfg1 S1),
   subst_inv.wf_State (value_id (getPhiNodeID (PEI_p pi))) (PEI_v pi) (PEI_f pi) 
     cfg1 S1'.
-Admitted.
+Proof.
 
+Local Opaque inscope_of_tmn inscope_of_cmd.
+
+  intros.
+  (sInsn_cases (induction HsInsn) Case); destruct TD as [los nts]; simpl HwfS1.
+
+Case "sReturn".
+Focus.
+
+  destruct_ctx_return.
+
+  remember (inscope_of_cmd F' (block_intro l2 ps2 (cs2' ++ c' :: cs') tmn') c')
+    as R2.
+  destruct R2; try solve [inversion Hinscope2].
+  remember (inscope_of_tmn F
+             (block_intro l1 ps1 (cs1' ++ nil)(insn_return rid RetTy Result))
+             (insn_return rid RetTy Result)) as R1.
+  destruct R1; try solve [inversion Hinscope1].
+  split; auto.
+    unfold wf_ExecutionContext. simpl.
+    remember (getCmdID c') as R.
+    destruct_cmd c'; try solve [inversion H].
+    assert (uniqFdef F') as HuniqF.
+      eapply wf_system__uniqFdef; eauto.
+    assert (wf_fdef S (module_intro los nts Ps) F') as HwfF.
+      eapply wf_system__wf_fdef; eauto.
+
+    assert (NoDup (getBlockLocs 
+                     (block_intro l2 ps2
+                        (cs2' ++ insn_call i0 n c t0 v0 v p :: cs') tmn'))) 
+      as Hnotin.
+      eapply wf_system__uniq_block with (f:=F') in HwfSystem; eauto.
+    destruct cs'; simpl_env in *.
+    SSSCase "1.1.1".
+        assert (HeqR2':=HeqR2).
+        apply inscope_of_cmd_tmn in HeqR2; auto.
+        destruct HeqR2 as [ids2 [J1 J2]].
+        rewrite <- J1.
+        unfold Opsem.returnUpdateLocals in H1. simpl in H1.
+        remember (Opsem.getOperandValue (los,nts) Result lc gl) as R1.
+        destruct R1; try solve [inv H1].
+        destruct R.
+          destruct n; inv HeqR.
+          remember (lift_op1 DGVs (fit_gv (los, nts) t0) g t0) as R2.
+          destruct R2; inv H1.
+          change i0 with
+            (getCmdLoc (insn_call i0 false c t0 v0 v p)); auto.
+          eapply wf_defs_updateAddAL; try solve [eauto | simpl; congruence].
+            simpl. apply in_middle.
+
+          destruct n; inv HeqR. inv H1.
+          simpl in J2.
+          eapply wf_defs_eq; eauto.
+
+    SSSCase "1.1.2".
+        assert (HeqR2':=HeqR2).
+        apply inscope_of_cmd_cmd in HeqR2; auto.
+        destruct HeqR2 as [ids2 [J1 J2]].
+        rewrite <- J1.
+        unfold Opsem.returnUpdateLocals in H1. simpl in H1.
+        remember (Opsem.getOperandValue (los,nts) Result lc gl) as R1.
+        destruct R1; try solve [inv H1].
+        destruct R.
+          destruct n; inv HeqR.
+          remember (lift_op1 DGVs (fit_gv (los, nts) t0) g t0) as R2.
+          destruct R2; inv H1.
+          change i0 with
+            (getCmdLoc (insn_call i0 false c t0 v0 v p)); auto.
+          eapply wf_defs_updateAddAL; try solve [eauto | simpl; congruence].
+            simpl. apply in_middle.
+
+          destruct n; inv HeqR. inv H1.
+          simpl in J2.
+          eapply wf_defs_eq; eauto.
+
+Unfocus.
+
+Case "sReturnVoid".
+Focus.
+
+  destruct_ctx_return.
+
+  remember (inscope_of_cmd F' (block_intro l2 ps2 (cs2' ++ c' :: cs') tmn') c')
+    as R2.
+  destruct R2; try solve [inversion Hinscope2].
+  remember (inscope_of_tmn F
+             (block_intro l1 ps1 (cs1' ++ nil)(insn_return_void rid))
+             (insn_return_void rid)) as R1.
+  destruct R1; try solve [inversion Hinscope1].
+  split; auto.
+    unfold wf_ExecutionContext. simpl.
+    apply HwfCall' in HBinF1. simpl in HBinF1.
+    assert (NoDup (getBlockLocs 
+                     (block_intro l2 ps2 (cs2' ++ c' :: cs') tmn'))) 
+      as Hnotin.
+      eapply wf_system__uniq_block with (f:=F') in HwfSystem; eauto.
+    destruct cs'; simpl_env in *.
+    SSSCase "1.1.1".
+        clear - HeqR2 Hinscope2 H HwfCall' HBinF1 Hnotin H1 Hinscope2'.
+        apply inscope_of_cmd_tmn in HeqR2; auto.
+        destruct HeqR2 as [ids2 [J1 J2]].
+        rewrite <- J1.
+        remember (getCmdID c') as R.
+        destruct_cmd c'; try solve [inversion H].
+        destruct n; inversion H1.
+        simpl in HeqR. subst R.
+        eapply wf_defs_eq; eauto.
+
+    SSSCase "1.1.2".
+        clear - HeqR2 Hinscope2 H HwfCall' HBinF1 Hnotin H1 Hinscope2'.
+        apply inscope_of_cmd_cmd in HeqR2; auto.
+        destruct HeqR2 as [ids2 [J1 J2]].
+        rewrite <- J1.
+        remember (getCmdID c') as R.
+        destruct_cmd c'; try solve [inversion H].
+        destruct n; inversion H1.
+        simpl in HeqR. subst R.
+        eapply wf_defs_eq; eauto.
+
+Unfocus.
+
+Case "sBranch".
+Focus.
+
+  destruct_ctx_other.
+  remember (inscope_of_tmn F
+             (block_intro l1' ps1' (cs1' ++ nil)(insn_br bid Cond l1 l2))
+             (insn_br bid Cond l1 l2)) as R1.
+  destruct R1; try solve [inversion Hinscope1].
+  split; auto.
+    unfold wf_ExecutionContext. simpl.
+    assert (HwfF := HwfSystem).
+    eapply wf_system__wf_fdef with (f:=F) in HwfF; eauto.
+    assert (HuniqF := HwfSystem).
+    eapply wf_system__uniqFdef with (f:=F) in HuniqF; eauto.
+    eapply inscope_of_tmn_br in HeqR1; eauto.
+    destruct HeqR1 as [ids0' [HeqR1 [J1 J2]]].
+    destruct cs'; rewrite <- HeqR1; auto.
+Unfocus.
+
+Case "sBranch_uncond".
+Focus.
+
+  destruct_ctx_other.
+  remember (inscope_of_tmn F
+             (block_intro l1' ps1' (cs1' ++ nil)(insn_br_uncond bid l0))
+             (insn_br_uncond bid l0)) as R1.
+  destruct R1; try solve [inversion Hinscope1].
+  split; auto.
+    unfold wf_ExecutionContext. simpl.
+    assert (HwfF := HwfSystem).
+    eapply wf_system__wf_fdef with (f:=F) in HwfF; eauto.
+    assert (HuniqF := HwfSystem).
+    eapply wf_system__uniqFdef with (f:=F) in HuniqF; eauto.
+    eapply inscope_of_tmn_br_uncond with (cs':=cs')(l':=l')(ps':=ps')
+      (tmn':=tmn') in HeqR1; eauto.
+    destruct HeqR1 as [ids0' [HeqR1 [J1 J2]]].
+    destruct cs'; rewrite <- HeqR1; auto.
+Unfocus.
+
+Case "sBop". abstract (eapply preservation_cmd_updated_case; eauto; auto).
+Case "sFBop".
+  abstract (eapply preservation_cmd_updated_case; eauto; auto).
+Case "sExtractValue".
+  abstract (eapply preservation_cmd_updated_case; eauto; simpl; eauto).
+Case "sInsertValue".
+  abstract (eapply preservation_cmd_updated_case; eauto; simpl; eauto).
+Case "sMalloc".
+  abstract (eapply preservation_cmd_updated_case; eauto; simpl; eauto 10).
+Case "sFree".
+  abstract (eapply preservation_cmd_non_updated_case; eauto; simpl; auto).
+Case "sAlloca".
+  abstract (eapply preservation_cmd_updated_case; eauto; simpl; eauto 10).
+Case "sLoad".
+  abstract (eapply preservation_cmd_updated_case; eauto; simpl; eauto 7).
+Case "sStore".
+  abstract (eapply preservation_cmd_non_updated_case; eauto; simpl; auto).
+Case "sGEP".
+  abstract (eapply preservation_cmd_updated_case; eauto; simpl; eauto 9).
+Case "sTrunc". abstract (eapply preservation_cmd_updated_case; eauto; auto).
+Case "sExt". abstract (eapply preservation_cmd_updated_case; eauto; auto).
+Case "sCast". abstract (eapply preservation_cmd_updated_case; eauto; auto).
+Case "sIcmp". abstract (eapply preservation_cmd_updated_case; eauto; auto).
+Case "sFcmp". abstract (eapply preservation_cmd_updated_case; eauto; auto).
+Case "sSelect".
+  abstract (
+    destruct (isGVZero (los, nts) c);
+      eapply preservation_cmd_updated_case; eauto; auto
+  ).
+
+Case "sCall".
+Focus.
+  destruct_ctx_other.
+
+  assert (InProductsB (product_fdef (fdef_intro
+    (fheader_intro fa rt fid la va) lb)) Ps = true) as HFinPs'.
+    apply OpsemAux.lookupFdefViaPtr_inversion in H1.
+    destruct H1 as [fn [H11 H12]].
+    eapply lookupFdefViaIDFromProducts_inv; eauto.
+
+  repeat (split; auto).
+    assert (uniqFdef (fdef_intro (fheader_intro fa rt fid la va) lb)) as Huniq.
+      eapply wf_system__uniqFdef; eauto.
+    assert (wf_fdef S (module_intro los nts Ps) 
+      (fdef_intro (fheader_intro fa rt fid la va) lb)) as HwfF.
+      eapply wf_system__wf_fdef; eauto.
+    unfold wf_ExecutionContext. simpl.
+    assert (ps'=nil) as EQ.
+      eapply entryBlock_has_no_phinodes with (s:=S); eauto.
+    subst.
+    apply dom_entrypoint in H2.
+
+Transparent inscope_of_tmn inscope_of_cmd.
+
+    destruct cs'.
+      unfold inscope_of_tmn.
+      remember ((dom_analyze (fdef_intro (fheader_intro fa rt fid la va) lb))
+        !! l') as R.
+      destruct R. simpl in H2. subst. simpl.
+      eapply preservation_dbCall_case; eauto.
+
+      unfold inscope_of_cmd, inscope_of_id.
+      rewrite init_scope_spec1; auto.
+      remember ((dom_analyze (fdef_intro (fheader_intro fa rt fid la va) lb))
+        !! l') as R.
+      destruct R. simpl. simpl in H2. subst. simpl.
+      destruct (eq_atom_dec (getCmdLoc c) (getCmdLoc c)) as [|n];
+        try solve [contradict n; auto].
+      eapply preservation_dbCall_case; eauto.
+Unfocus.
+
+Case "sExCall".
+  abstract (
+  match goal with
+  | H5: Opsem.exCallUpdateLocals _ _ _ _ _ _ = _ |- _ =>
+    unfold Opsem.exCallUpdateLocals in H5;
+    destruct noret0; try solve [
+      inv H5; eapply preservation_cmd_non_updated_case in HwfS1; eauto; auto |
+      destruct oresult; tinv H5;
+      remember (fit_gv (los, nts) rt1 g) as R;
+      destruct R; inv H5;
+      eapply preservation_cmd_updated_case with (Mem1:=Mem') in HwfS1; 
+        simpl; eauto; simpl; auto]
+  end).
+Qed.
+
+(* similar to id_rhs_val *)
+Lemma initLocals__wf_defs : forall pi fid l' fa rt la va
+  lb gvs lc CurLayouts CurNamedts initGlobal 
+  (Huniq: uniqFdef (fdef_intro (fheader_intro fa rt fid la va) lb))
+  (Hinit : Opsem.initLocals
+     (OpsemAux.initTargetData CurLayouts CurNamedts Mem.empty)
+     la gvs = Some lc),
+   match
+     fold_left
+       (inscope_of_block (fdef_intro (fheader_intro fa rt fid la va) lb) l')
+       nil (ret getArgsIDs la)
+   with
+   | ret ids0 =>
+       wf_defs (value_id (getPhiNodeID (PEI_p pi))) (PEI_v pi) (PEI_f pi)
+         (OpsemAux.initTargetData CurLayouts CurNamedts Mem.empty) initGlobal
+         (fdef_intro (fheader_intro fa rt fid la va) lb) lc ids0
+   | merror => False
+   end.
+Proof.
+  intros.
+  assert (incl nil (bound_blocks lb)) as J.
+    intros x J. inv J.
+  apply fold_left__bound_blocks with (fh:=fheader_intro fa rt fid la va)(l0:=l')
+    (init:=getArgsIDs la) in J.
+  destruct J as [r J]. unfold l in *.
+  intros EQ gvs1 gvs2 Hinscope1 Hget1 Hget2.
+  assert (uniqFdef (PEI_f pi)) as Huniq'. 
+    rewrite EQ. auto.
+  simpl in *. uniq_result.
+  contradict Hinscope1.
+  apply PEInfo_p__isnt__arg in Huniq'.
+  rewrite EQ in Huniq'. auto.
+Qed.
+
+(* similar to id_rhs_val *)
 Lemma s_genInitState__inv: forall (S : system) (main : id) (pi: PEInfo) 
   (VarArgs : list (GVsT DGVs)) (cfg : OpsemAux.Config) (IS : Opsem.State)
   (HwfS: wf_system S)
   (Hinit: Opsem.s_genInitState S main VarArgs Mem.empty = ret (cfg, IS)),
   wf_State (value_id (getPhiNodeID (PEI_p pi))) (PEI_v pi) (PEI_f pi) cfg IS.
-Admitted.
+Proof.
+  intros.
+  simpl_s_genInitState.
+Local Opaque inscope_of_tmn inscope_of_cmd.
+  simpl.
+  split; auto.
+    apply getParentOfFdefFromSystem__moduleInProductsInSystemB in HeqR0.
+    destruct HeqR0 as [HMinS HinPs].
+    assert (uniqFdef (fdef_intro (fheader_intro f t i0 a v) b)) as Huniq.
+      eapply wf_system__uniqFdef; eauto.
+    unfold wf_ExecutionContext. simpl.
+    assert (ps0=nil) as EQ.
+      eapply entryBlock_has_no_phinodes with (s:=S); eauto.        
+    subst.
+Transparent inscope_of_tmn inscope_of_cmd.
+    apply dom_entrypoint in HeqR2.
+    destruct cs0.
+      unfold inscope_of_tmn.
+      remember ((dom_analyze (fdef_intro (fheader_intro f t i0 a v) b))
+        !! l0) as R.
+      destruct R. simpl in HeqR2. subst.
+      eapply initLocals__wf_defs; eauto.
+
+      unfold inscope_of_cmd, inscope_of_id.
+      rewrite init_scope_spec1; auto.
+      remember ((dom_analyze (fdef_intro (fheader_intro f t i0 a v) b))
+        !! l0) as R.
+      destruct R. simpl. simpl in HeqR2. subst.
+      destruct (eq_atom_dec (getCmdLoc c) (getCmdLoc c)) as [|n];
+        try solve [contradict n; auto].
+      eapply initLocals__wf_defs; eauto.
+Qed.
+
